Started documenting the theories.

src/Run.thy
@@ -5,10 +5,10 @@ imports TESL
       
 begin
 text \<open>
-  Runs are sequences of instants, each instant mapping a clock to a pair that whether the clock 
-  ticks or not and what is the current time on this clock. The first element of the pair is
-  called the \<^emph>\<open>hamlet\<close> of the clock (to tick or not to tick), the second element is called the 
-  \<^emph>\<open>time\<close>.
+  Runs are sequences of instants, and each instant maps a clock to a pair that 
+  tells whether the clock ticks or not, and what is the current time on this clock.
+  The first element of the pair is called the \<^emph>\<open>hamlet\<close> of the clock (to tick or 
+  not to tick), the second element is called the \<^emph>\<open>time\<close>.
 \<close>
 
 abbreviation hamlet where \<open>hamlet \<equiv> fst\<close>
@@ -17,8 +17,9 @@ abbreviation time   where \<open>time \<equiv> snd\<close>
 type_synonym '\<tau> instant = \<open>clock \<Rightarrow> (bool \<times> '\<tau> tag_const)\<close>
 
 text\<open>
-  Runs have the additional constraint that time cannot go backwards on any clock in the sequence 
-  of instants. Therefore, for any clock, the time projection of a run is monotonous.
+  Runs have the additional constraint that time cannot go backwards on any clock
+  in the sequence of instants.
+Therefore, for any clock, the time projection of a run is monotonous.
 \<close>
 typedef (overloaded) '\<tau>::linordered_field run =
   \<open>{ \<rho>::nat \<Rightarrow> '\<tau> instant. \<forall>c. mono (\<lambda>n. time (\<rho> n c)) }\<close>
@@ -29,33 +30,46 @@ qed
 
 lemma Abs_run_inverse_rewrite:
   \<open>\<forall>c. mono (\<lambda>n. time (\<rho> n c)) \<Longrightarrow> Rep_run (Abs_run \<rho>) = \<rho>\<close>
-  by (simp add: Abs_run_inverse)
+by (simp add: Abs_run_inverse)
 
 text\<open>
   @{term \<open>run_tick_count \<rho> K n\<close>} counts the number of ticks on clock @{term \<open>K\<close>} 
   in the interval \<^verbatim>\<open>[0, n]\<close> of run @{term \<open>\<rho>\<close>}.
 \<close>
-fun run_tick_count :: \<open>('\<tau>::linordered_field) run \<Rightarrow> clock \<Rightarrow> nat \<Rightarrow> nat\<close> ("#\<^sub>\<le> _ _ _") where
-    \<open>(#\<^sub>\<le> \<rho> K 0)       = (if hamlet ((Rep_run \<rho>) 0 K)
-                         then 1
-                         else 0)\<close>
-  | \<open>(#\<^sub>\<le> \<rho> K (Suc n)) = (if hamlet ((Rep_run \<rho>) (Suc n) K)
-                         then 1 + (#\<^sub>\<le> \<rho> K n)
-                         else (#\<^sub>\<le> \<rho> K n))\<close>
+fun run_tick_count :: \<open>('\<tau>::linordered_field) run \<Rightarrow> clock \<Rightarrow> nat \<Rightarrow> nat\<close>
+  ("#\<^sub>\<le> _ _ _")
+where
+  \<open>(#\<^sub>\<le> \<rho> K 0)       = (if hamlet ((Rep_run \<rho>) 0 K)
+                       then 1
+                       else 0)\<close>
+| \<open>(#\<^sub>\<le> \<rho> K (Suc n)) = (if hamlet ((Rep_run \<rho>) (Suc n) K)
+                       then 1 + (#\<^sub>\<le> \<rho> K n)
+                       else (#\<^sub>\<le> \<rho> K n))\<close>
 
 text\<open>
-  @{term \<open>run_tick_count_strictly \<rho> K n\<close>} counts the number of ticks on clock @{term \<open>K\<close>} 
-  in the interval \<^verbatim>\<open>[0, n[\<close> of run @{term \<open>\<rho>\<close>}.
+  @{term \<open>run_tick_count_strictly \<rho> K n\<close>} counts the number of ticks on
+  clock @{term \<open>K\<close>} in the interval \<^verbatim>\<open>[0, n[\<close> of run @{term \<open>\<rho>\<close>}.
 \<close>
-fun run_tick_count_strictly :: \<open>('\<tau>::linordered_field) run \<Rightarrow> clock \<Rightarrow> nat \<Rightarrow> nat\<close> ("#\<^sub>< _ _ _")
+fun run_tick_count_strictly :: \<open>('\<tau>::linordered_field) run \<Rightarrow> clock \<Rightarrow> nat \<Rightarrow> nat\<close>
+  ("#\<^sub>< _ _ _")
 where
-    \<open>(#\<^sub>< \<rho> K 0)       = 0\<close>
-  | \<open>(#\<^sub>< \<rho> K (Suc n)) = #\<^sub>\<le> \<rho> K n\<close>
+  \<open>(#\<^sub>< \<rho> K 0)       = 0\<close>
+| \<open>(#\<^sub>< \<rho> K (Suc n)) = #\<^sub>\<le> \<rho> K n\<close>
 
-definition first_time :: \<open>'a::linordered_field run \<Rightarrow> clock \<Rightarrow> nat \<Rightarrow> 'a tag_const \<Rightarrow> bool\<close>
+text\<open>
+  @{term \<open>first_time \<rho> K n \<tau>\<close>} tells whether instant @{term \<open>n\<close>} in run @{term\<open>\<rho>\<close>}
+  is the first one where the time on clock @{term \<open>K\<close>} reaches @{term \<open>\<tau>\<close>}.
+\<close>
+definition first_time :: \<open>'a::linordered_field run \<Rightarrow> clock \<Rightarrow> nat \<Rightarrow> 'a tag_const
+                          \<Rightarrow> bool\<close>
 where
-  \<open>first_time \<rho> K n \<tau> \<equiv> (time ((Rep_run \<rho>) n K) = \<tau>) \<and> (\<nexists>n'. n' < n \<and> time ((Rep_run \<rho>) n' K) = \<tau>)\<close>
+  \<open>first_time \<rho> K n \<tau> \<equiv> (time ((Rep_run \<rho>) n K) = \<tau>)
+                      \<and> (\<nexists>n'. n' < n \<and> time ((Rep_run \<rho>) n' K) = \<tau>)\<close>
 
+text\<open>
+  The time on a clock is necessarily less than @{term \<open>\<tau>\<close>} before the first instant
+  at which it reaches @{term \<open>\<tau>\<close>}.
+\<close>
 lemma before_first_time:
   assumes \<open>first_time \<rho> K n \<tau>\<close>
       and \<open>m < n\<close>
@@ -64,18 +78,25 @@ proof -
   have \<open>mono (\<lambda>n. time (Rep_run \<rho> n K))\<close> using Rep_run by blast
   moreover from assms(2) have \<open>m \<le> n\<close> using less_imp_le by simp
   moreover have \<open>mono (\<lambda>n. time (Rep_run \<rho> n K))\<close> using Rep_run by blast
-  ultimately have  \<open>time ((Rep_run \<rho>) m K) \<le> time ((Rep_run \<rho>) n K)\<close> by (simp add:mono_def)
-  moreover from assms(1) have \<open>time ((Rep_run \<rho>) n K) = \<tau>\<close> using first_time_def by blast
-  moreover from assms have \<open>time ((Rep_run \<rho>) m K) \<noteq> \<tau>\<close> using first_time_def by blast
+  ultimately have  \<open>time ((Rep_run \<rho>) m K) \<le> time ((Rep_run \<rho>) n K)\<close>
+    by (simp add:mono_def)
+  moreover from assms(1) have \<open>time ((Rep_run \<rho>) n K) = \<tau>\<close>
+    using first_time_def by blast
+  moreover from assms have \<open>time ((Rep_run \<rho>) m K) \<noteq> \<tau>\<close>
+    using first_time_def by blast
   ultimately show ?thesis by simp
 qed
 
+text\<open>
+  This leads to an alternate definition of @{term \<open>first_time\<close>}:
+\<close>
 lemma alt_first_time_def:
   assumes \<open>\<forall>m < n. time ((Rep_run \<rho>) m K) < \<tau>\<close>
       and \<open>time ((Rep_run \<rho>) n K) = \<tau>\<close>
     shows \<open>first_time \<rho> K n \<tau>\<close>
 proof -
-  from assms(1) have \<open>\<forall>m < n. time ((Rep_run \<rho>) m K) \<noteq> \<tau>\<close> by (simp add: less_le)
+  from assms(1) have \<open>\<forall>m < n. time ((Rep_run \<rho>) m K) \<noteq> \<tau>\<close>
+    by (simp add: less_le)
   with assms(2) show ?thesis by (simp add: first_time_def)
 qed
 
