src/SymbolicPrimitive.thy
@@ -1,41 +1,96 @@
+chapter \<open>Symbolic Primitives for Building Runs\<close>
+
 theory SymbolicPrimitive
   imports Run
 
 begin
+
+text\<open>
+  We define here the primitive constraints on runs toward which we will translate
+  TESL specifications in the operational semantics.
+  These constraints refer to a specific symbolic run and can therefore access
+  properties of the run at particular instants (for instance, the fact that a clock
+  ticks at instant @{term \<open>n\<close>} of the run, or the time on a given clock at 
+  that instant).
+
+  In the previous chapters, we had no reference to particular instants of a run 
+  because the TESL language should be invariant by stuttering in order to allow 
+  the composition of specifications: adding an instant where no clock ticks to 
+  a run that satisfies a formula should yield another satisfying run. However, 
+  when constructing runs that satisfy a formula, we need to be able to refer to 
+  the time or hamlet of a clock at a given instant.
+\<close>
+
+text\<open>
+  Counter expressions are used to get the number of ticks of a clock up to 
+  (strictly or not) a given instant index.
+\<close>
 datatype cnt_expr =
   TickCountLess \<open>clock\<close> \<open>instant_index\<close> ("#\<^sup><")
 | TickCountLeq \<open>clock\<close> \<open>instant_index\<close>  ("#\<^sup>\<le>")
 
 subsection\<open> Symbolic Primitives for Runs \<close>
 
+text\<open>
+  Tag variables are used to get the time on a clock at a given instant index.
+\<close>
 datatype tag_var =
   TSchematic \<open>clock * instant_index\<close> ("\<tau>\<^sub>v\<^sub>a\<^sub>r")
 
 datatype '\<tau> constr =
+\<comment> \<open>@{term \<open>c \<Down> n @ \<tau>\<close>} constrains clock @{term \<open>c\<close>} to have time @{term \<open>\<tau>\<close>}
+    at instant @{term \<open>n\<close>} of the run.\<close>
   Timestamp     \<open>clock\<close>   \<open>instant_index\<close> \<open>'\<tau> tag_const\<close>         ("_ \<Down> _ @ _")
+\<comment> \<open>@{term \<open>m @ n \<oplus> \<delta>t \<Rightarrow> s\<close>} constrains clock @{term \<open>s\<close>} to tick at the
+    first instant at which the time on @{term \<open>m\<close>} has increased by @{term \<open>\<delta>t\<close>}
+    from the value it had at instant @{term \<open>n\<close>} of the run.\<close>
 | TimeDelay     \<open>clock\<close>   \<open>instant_index\<close> \<open>'\<tau> tag_const\<close> \<open>clock\<close> ("_ @ _ \<oplus> _ \<Rightarrow> _")
+\<comment> \<open>@{term \<open>c \<Up> n\<close>} constrains clock @{term \<open>c\<close>} to tick
+    at instant @{term \<open>n\<close>} of the run.\<close>
 | Ticks         \<open>clock\<close>   \<open>instant_index\<close>                        ("_ \<Up> _")
+\<comment> \<open>@{term \<open>c \<not>\<Up> n\<close>} constrains clock @{term \<open>c\<close>} not to tick
+    at instant @{term \<open>n\<close>} of the run.\<close>
 | NotTicks      \<open>clock\<close>   \<open>instant_index\<close>                        ("_ \<not>\<Up> _")
+\<comment> \<open>@{term \<open>c \<not>\<Up> < n\<close>} constrains clock @{term \<open>c\<close>} not to tick
+    before instant @{term \<open>n\<close>} of the run.\<close>
 | NotTicksUntil \<open>clock\<close>   \<open>instant_index\<close>                        ("_ \<not>\<Up> < _")
+\<comment> \<open>@{term \<open>c \<not>\<Up> \<ge> n\<close>} constrains clock @{term \<open>c\<close>} not to tick
+    at and after instant @{term \<open>n\<close>} of the run.\<close>
 | NotTicksFrom  \<open>clock\<close>   \<open>instant_index\<close>                        ("_ \<not>\<Up> \<ge> _")
+\<comment> \<open>@{term \<open>\<lfloor>\<tau>\<^sub>1, \<tau>\<^sub>2\<rfloor> \<in> R\<close>} constrains tag variables @{term \<open>\<tau>\<^sub>1\<close>} and  @{term \<open>\<tau>\<^sub>2\<close>} 
+    to be in relation @{term \<open>R\<close>}.\<close>
 | TagArith      \<open>tag_var\<close> \<open>tag_var\<close> \<open>('\<tau> tag_const \<times> '\<tau> tag_const) \<Rightarrow> bool\<close> ("\<lfloor>_, _\<rfloor> \<in> _")
+\<comment> \<open>@{term \<open>\<lceil>k\<^sub>1, k\<^sub>2\<rceil> \<in> R\<close>} constrains counter expressions @{term \<open>k\<^sub>1\<close>} and  @{term \<open>k\<^sub>2\<close>} 
+    to be in relation @{term \<open>R\<close>}.\<close>
 | TickCntArith  \<open>cnt_expr\<close> \<open>cnt_expr\<close> \<open>(nat \<times> nat) \<Rightarrow> bool\<close>      ("\<lceil>_, _\<rceil> \<in> _")
+\<comment> \<open>@{term \<open>k\<^sub>1 \<preceq> k\<^sub>2\<close>} constrains counter expression @{term \<open>k\<^sub>1\<close>} to be less or equal 
+    to counter expression @{term \<open>k\<^sub>2\<close>}.\<close>
 | TickCntLeq    \<open>cnt_expr\<close> \<open>cnt_expr\<close>                            ("_ \<preceq> _")
 
 type_synonym '\<tau> system = \<open>'\<tau> constr list\<close>
 
 
-\<comment> \<open>
-  The abstract machine follows the intuition: 
-    past [@term\<open>\<Gamma>\<close>], current index [n], present [@term\<open>\<Psi>\<close>], future [@term\<open>\<Phi>\<close>]
-   Beware: This type is slightly different from the one originally implemented in Heron
+text \<open>
+  The abstract machine has configurations composed of:
+  \<^item> the past @{term\<open>\<Gamma>\<close>}, which captures choices that have already be made as a 
+    list of symbolic primitive constraints on the run;
+  \<^item> the current index @{term \<open>n\<close>}, which is the index of the present instant;
+  \<^item> the present @{term\<open>\<Psi>\<close>}, which captures the formulae that must be satisfied
+    in the current instant;
+  \<^item> the future @{term\<open>\<Phi>\<close>}, which captures the constraints on the future of the run.
 \<close>
-type_synonym '\<tau> config = \<open>'\<tau> system * instant_index * '\<tau> TESL_formula * '\<tau> TESL_formula\<close>
+type_synonym '\<tau> config =
+                \<open>'\<tau> system * instant_index * '\<tau> TESL_formula * '\<tau> TESL_formula\<close>
 
 
 section \<open>Semantics of Primitive Constraints \<close>
 
-fun counter_expr_eval :: \<open>('\<tau>::linordered_field) run \<Rightarrow> cnt_expr \<Rightarrow> nat\<close> ("\<lbrakk> _ \<turnstile> _ \<rbrakk>\<^sub>c\<^sub>n\<^sub>t\<^sub>e\<^sub>x\<^sub>p\<^sub>r")
+text\<open>
+  The semantics of the primitive constraints is defined in a way similar to
+  the semantics of TESL formulae.
+\<close>
+fun counter_expr_eval :: \<open>('\<tau>::linordered_field) run \<Rightarrow> cnt_expr \<Rightarrow> nat\<close>
+  ("\<lbrakk> _ \<turnstile> _ \<rbrakk>\<^sub>c\<^sub>n\<^sub>t\<^sub>e\<^sub>x\<^sub>p\<^sub>r")
 where
   \<open>\<lbrakk> \<rho> \<turnstile> #\<^sup>< clk indx \<rbrakk>\<^sub>c\<^sub>n\<^sub>t\<^sub>e\<^sub>x\<^sub>p\<^sub>r = run_tick_count_strictly \<rho> clk indx\<close>
 | \<open>\<lbrakk> \<rho> \<turnstile> #\<^sup>\<le> clk indx \<rbrakk>\<^sub>c\<^sub>n\<^sub>t\<^sub>e\<^sub>x\<^sub>p\<^sub>r = run_tick_count \<rho> clk indx\<close>
@@ -45,8 +100,9 @@ fun symbolic_run_interpretation_primitive
   ::\<open>('\<tau>::linordered_field) constr \<Rightarrow> '\<tau> run set\<close> ("\<lbrakk> _ \<rbrakk>\<^sub>p\<^sub>r\<^sub>i\<^sub>m")
 where
   \<open>\<lbrakk> K \<Up> n  \<rbrakk>\<^sub>p\<^sub>r\<^sub>i\<^sub>m     = {\<rho>. hamlet ((Rep_run \<rho>) n K) }\<close>
-| \<open>\<lbrakk> K @ n\<^sub>0 \<oplus> \<delta>t \<Rightarrow> K' \<rbrakk>\<^sub>p\<^sub>r\<^sub>i\<^sub>m = {\<rho>. \<forall>n \<ge> n\<^sub>0. first_time \<rho> K n (time ((Rep_run \<rho>) n\<^sub>0 K) + \<delta>t)
-                                            \<longrightarrow> hamlet ((Rep_run \<rho>) n K')}\<close>
+| \<open>\<lbrakk> K @ n\<^sub>0 \<oplus> \<delta>t \<Rightarrow> K' \<rbrakk>\<^sub>p\<^sub>r\<^sub>i\<^sub>m =
+                  {\<rho>. \<forall>n \<ge> n\<^sub>0. first_time \<rho> K n (time ((Rep_run \<rho>) n\<^sub>0 K) + \<delta>t)
+                               \<longrightarrow> hamlet ((Rep_run \<rho>) n K')}\<close>
 | \<open>\<lbrakk> K \<not>\<Up> n \<rbrakk>\<^sub>p\<^sub>r\<^sub>i\<^sub>m     = {\<rho>. \<not>hamlet ((Rep_run \<rho>) n K) }\<close>
 | \<open>\<lbrakk> K \<not>\<Up> < n \<rbrakk>\<^sub>p\<^sub>r\<^sub>i\<^sub>m   = {\<rho>. \<forall>i < n. \<not> hamlet ((Rep_run \<rho>) i K)}\<close>
 | \<open>\<lbrakk> K \<not>\<Up> \<ge> n \<rbrakk>\<^sub>p\<^sub>r\<^sub>i\<^sub>m   = {\<rho>. \<forall>i \<ge> n. \<not> hamlet ((Rep_run \<rho>) i K) }\<close>
@@ -56,10 +112,15 @@ where
 | \<open>\<lbrakk> \<lceil>e\<^sub>1, e\<^sub>2\<rceil> \<in> R \<rbrakk>\<^sub>p\<^sub>r\<^sub>i\<^sub>m = { \<rho>. R (\<lbrakk> \<rho> \<turnstile> e\<^sub>1 \<rbrakk>\<^sub>c\<^sub>n\<^sub>t\<^sub>e\<^sub>x\<^sub>p\<^sub>r, \<lbrakk> \<rho> \<turnstile> e\<^sub>2 \<rbrakk>\<^sub>c\<^sub>n\<^sub>t\<^sub>e\<^sub>x\<^sub>p\<^sub>r) }\<close>
 | \<open>\<lbrakk> cnt_e\<^sub>1 \<preceq> cnt_e\<^sub>2 \<rbrakk>\<^sub>p\<^sub>r\<^sub>i\<^sub>m = { \<rho>. \<lbrakk> \<rho> \<turnstile> cnt_e\<^sub>1 \<rbrakk>\<^sub>c\<^sub>n\<^sub>t\<^sub>e\<^sub>x\<^sub>p\<^sub>r \<le> \<lbrakk> \<rho> \<turnstile> cnt_e\<^sub>2 \<rbrakk>\<^sub>c\<^sub>n\<^sub>t\<^sub>e\<^sub>x\<^sub>p\<^sub>r }\<close>
 
+text\<open>
+  The composition of primitive constraints is their conjunction, and we get the
+  set of satisfying runs by intersection.
+\<close>
 fun symbolic_run_interpretation
-  ::\<open>('\<tau>::linordered_field) constr list \<Rightarrow> ('\<tau>::linordered_field) run set\<close> ("\<lbrakk>\<lbrakk> _ \<rbrakk>\<rbrakk>\<^sub>p\<^sub>r\<^sub>i\<^sub>m")
+  ::\<open>('\<tau>::linordered_field) constr list \<Rightarrow> ('\<tau>::linordered_field) run set\<close>
+  ("\<lbrakk>\<lbrakk> _ \<rbrakk>\<rbrakk>\<^sub>p\<^sub>r\<^sub>i\<^sub>m")
 where
-  \<open>\<lbrakk>\<lbrakk> [] \<rbrakk>\<rbrakk>\<^sub>p\<^sub>r\<^sub>i\<^sub>m = { _. True }\<close>
+  \<open>\<lbrakk>\<lbrakk> [] \<rbrakk>\<rbrakk>\<^sub>p\<^sub>r\<^sub>i\<^sub>m = {\<rho>. True }\<close>
 | \<open>\<lbrakk>\<lbrakk> \<gamma> # \<Gamma> \<rbrakk>\<rbrakk>\<^sub>p\<^sub>r\<^sub>i\<^sub>m = \<lbrakk> \<gamma> \<rbrakk>\<^sub>p\<^sub>r\<^sub>i\<^sub>m \<inter> \<lbrakk>\<lbrakk> \<Gamma> \<rbrakk>\<rbrakk>\<^sub>p\<^sub>r\<^sub>i\<^sub>m\<close>
 
 lemma symbolic_run_interp_cons_morph:
@@ -70,31 +131,37 @@ definition consistent_context :: \<open>('\<tau>::linordered_field) constr list 
 where 
   \<open>consistent_context \<Gamma> \<equiv> \<exists>\<rho>. \<rho> \<in> \<lbrakk>\<lbrakk> \<Gamma> \<rbrakk>\<rbrakk>\<^sub>p\<^sub>r\<^sub>i\<^sub>m\<close>
 
-subsection \<open>Defining a method for witness construction\<close> (**)
+subsection \<open>Defining a method for witness construction\<close>
 
-\<comment> \<open>Initial states\<close>
+text\<open>
+  In order to build a run, we can start from an initial run in which no clock 
+  ticks and the time is always 0 on any clock.
+\<close>
 abbreviation initial_run :: \<open>('\<tau>::linordered_field) run\<close> ("\<rho>\<^sub>\<odot>") where
   \<open>\<rho>\<^sub>\<odot> \<equiv> Abs_run ((\<lambda>_ _. (False, \<tau>\<^sub>c\<^sub>s\<^sub>t 0)) ::nat \<Rightarrow> clock \<Rightarrow> (bool \<times> '\<tau> tag_const))\<close>
 
-\<comment> \<open>To ensure monotonicity, time tag is set at a specific instant and forever after (stuttering)\<close>
+text\<open>
+  To help avoiding that time flows backward, setting the time on a clock at a given 
+  instant sets it for the future instants too.
+\<close>
 fun time_update
-  :: \<open>nat \<Rightarrow> clock \<Rightarrow> ('\<tau>::linordered_field) tag_const \<Rightarrow> (nat \<Rightarrow> clock \<Rightarrow> (bool \<times> '\<tau> tag_const))
-      \<Rightarrow> (nat \<Rightarrow> clock \<Rightarrow> (bool \<times> '\<tau> tag_const))\<close>
+  :: \<open>nat \<Rightarrow> clock \<Rightarrow> ('\<tau>::linordered_field) tag_const \<Rightarrow> (nat \<Rightarrow> '\<tau> instant)
+      \<Rightarrow> (nat \<Rightarrow> '\<tau> instant)\<close>
 where
-  \<open>time_update n K \<tau> \<rho> = (\<lambda>n' K'. if K = K' \<and> n \<le> n' then (hamlet (\<rho> n K), \<tau>) else \<rho> n' K')\<close>
+  \<open>time_update n K \<tau> \<rho> = (\<lambda>n' K'. if K = K' \<and> n \<le> n'
+                                  then (hamlet (\<rho> n K), \<tau>)
+                                  else \<rho> n' K')\<close>
 
 
-section \<open>Rules and properties of consistence\<close> (**)
-
-(* declare [[show_sorts]] *)
+section \<open>Rules and properties of consistence\<close>
 
 lemma context_consistency_preservationI:
-  \<open>consistent_context ((\<gamma> :: ('\<tau>::linordered_field) constr) # \<Gamma>) \<Longrightarrow> consistent_context \<Gamma>\<close>
-unfolding consistent_context_def
-by auto
+  \<open>consistent_context ((\<gamma>::('\<tau>::linordered_field) constr)#\<Gamma>) \<Longrightarrow> consistent_context \<Gamma>\<close>
+unfolding consistent_context_def by auto
 
 \<comment> \<open>This is very restrictive\<close>
-inductive context_independency::\<open>('\<tau>::linordered_field) constr \<Rightarrow> '\<tau> constr list \<Rightarrow> bool\<close> ("_ \<bowtie> _")
+inductive context_independency
+  ::\<open>('\<tau>::linordered_field) constr \<Rightarrow> '\<tau> constr list \<Rightarrow> bool\<close> ("_ \<bowtie> _")
 where
   NotTicks_independency:
   \<open>(K \<Up> n) \<notin> set \<Gamma> \<Longrightarrow> (K \<not>\<Up> n) \<bowtie> \<Gamma>\<close>
@@ -103,33 +170,22 @@ where
 | Timestamp_independency:
   \<open>(\<nexists>\<tau>'. \<tau>' = \<tau> \<and> (K \<Down> n @ \<tau>) \<in> set \<Gamma>) \<Longrightarrow> (K \<Down> n @ \<tau>) \<bowtie> \<Gamma>\<close>
 
-\<^cancel>\<open>
-lemma context_consistency_preservationE:
-  assumes consist: \<open>consistent_context \<Gamma>\<close>
-  and     indepen: \<open>\<gamma> \<bowtie> \<Gamma>\<close>
-  shows   \<open>consistent_context (\<gamma> # \<Gamma>)\<close>
-  oops
-\<close>
 
 section\<open>Major Theorems\<close>
 subsection \<open>Fixpoint lemma\<close>
 
 theorem symrun_interp_fixpoint:
   \<open>\<Inter> ((\<lambda>\<gamma>. \<lbrakk> \<gamma> \<rbrakk>\<^sub>p\<^sub>r\<^sub>i\<^sub>m) ` set \<Gamma>) = \<lbrakk>\<lbrakk> \<Gamma> \<rbrakk>\<rbrakk>\<^sub>p\<^sub>r\<^sub>i\<^sub>m\<close>
-proof (induct \<Gamma>)
-  case Nil thus ?case by simp
-next
-  case Cons thus ?case by auto
-qed
+by (induction \<Gamma>, simp+)
 
 subsection \<open>Expansion law\<close>
 text \<open>Similar to the expansion laws of lattices\<close>
 
 theorem symrun_interp_expansion:
   \<open>\<lbrakk>\<lbrakk> \<Gamma>\<^sub>1 @ \<Gamma>\<^sub>2 \<rbrakk>\<rbrakk>\<^sub>p\<^sub>r\<^sub>i\<^sub>m = \<lbrakk>\<lbrakk> \<Gamma>\<^sub>1 \<rbrakk>\<rbrakk>\<^sub>p\<^sub>r\<^sub>i\<^sub>m \<inter> \<lbrakk>\<lbrakk> \<Gamma>\<^sub>2 \<rbrakk>\<rbrakk>\<^sub>p\<^sub>r\<^sub>i\<^sub>m\<close>
-by (induction \<Gamma>\<^sub>1, auto)
+by (induction \<Gamma>\<^sub>1, simp, auto)
 
-section \<open>Equational laws for TESL formulae denotationally interpreted\<close> 
+section \<open>Equational laws for the interpretation of symbolic primitives\<close> 
 subsection \<open>General laws\<close>
 
 lemma symrun_interp_assoc:
@@ -170,7 +226,7 @@ lemma symrun_interp_neutral2:
   \<open>\<lbrakk>\<lbrakk> \<Gamma> @ [] \<rbrakk>\<rbrakk>\<^sub>p\<^sub>r\<^sub>i\<^sub>m = \<lbrakk>\<lbrakk> \<Gamma> \<rbrakk>\<rbrakk>\<^sub>p\<^sub>r\<^sub>i\<^sub>m\<close>
 by simp
 
-subsection \<open>Decreasing interpretation of TESL formulae\<close>
+subsection \<open>Decreasing interpretation of symbolic primitives\<close>
 
 lemma TESL_sem_decreases_head:
   \<open>\<lbrakk>\<lbrakk> \<Gamma> \<rbrakk>\<rbrakk>\<^sub>p\<^sub>r\<^sub>i\<^sub>m \<supseteq> \<lbrakk>\<lbrakk> \<gamma> # \<Gamma> \<rbrakk>\<rbrakk>\<^sub>p\<^sub>r\<^sub>i\<^sub>m\<close>
@@ -185,22 +241,17 @@ lemma symrun_interp_formula_stuttering:
     shows \<open>\<lbrakk>\<lbrakk> \<gamma> # \<Gamma> \<rbrakk>\<rbrakk>\<^sub>p\<^sub>r\<^sub>i\<^sub>m = \<lbrakk>\<lbrakk> \<Gamma> \<rbrakk>\<rbrakk>\<^sub>p\<^sub>r\<^sub>i\<^sub>m\<close>
 proof -
   have \<open>\<gamma> # \<Gamma> = [\<gamma>] @ \<Gamma>\<close> by simp
-  hence \<open>\<lbrakk>\<lbrakk> \<gamma> # \<Gamma> \<rbrakk>\<rbrakk>\<^sub>p\<^sub>r\<^sub>i\<^sub>m = \<lbrakk>\<lbrakk> [\<gamma>] \<rbrakk>\<rbrakk>\<^sub>p\<^sub>r\<^sub>i\<^sub>m \<inter> \<lbrakk>\<lbrakk> \<Gamma> \<rbrakk>\<rbrakk>\<^sub>p\<^sub>r\<^sub>i\<^sub>m\<close> using symrun_interp_expansion by simp
+  hence \<open>\<lbrakk>\<lbrakk> \<gamma> # \<Gamma> \<rbrakk>\<rbrakk>\<^sub>p\<^sub>r\<^sub>i\<^sub>m = \<lbrakk>\<lbrakk> [\<gamma>] \<rbrakk>\<rbrakk>\<^sub>p\<^sub>r\<^sub>i\<^sub>m \<inter> \<lbrakk>\<lbrakk> \<Gamma> \<rbrakk>\<rbrakk>\<^sub>p\<^sub>r\<^sub>i\<^sub>m\<close>
+    using symrun_interp_expansion by simp
   thus ?thesis using assms symrun_interp_fixpoint by fastforce
 qed
 
-lemma symrun_interp_decreases:
-  \<open>\<lbrakk>\<lbrakk> \<Gamma> \<rbrakk>\<rbrakk>\<^sub>p\<^sub>r\<^sub>i\<^sub>m \<supseteq> \<lbrakk>\<lbrakk> \<gamma> # \<Gamma> \<rbrakk>\<rbrakk>\<^sub>p\<^sub>r\<^sub>i\<^sub>m\<close>
-by (rule TESL_sem_decreases_head)
-
 lemma symrun_interp_remdups_absorb:
   \<open>\<lbrakk>\<lbrakk> \<Gamma> \<rbrakk>\<rbrakk>\<^sub>p\<^sub>r\<^sub>i\<^sub>m = \<lbrakk>\<lbrakk> remdups \<Gamma> \<rbrakk>\<rbrakk>\<^sub>p\<^sub>r\<^sub>i\<^sub>m\<close>
-proof (induct \<Gamma>)
-  case Nil thus ?case by simp
-next
+proof (induction \<Gamma>)
   case Cons
     thus ?case using symrun_interp_formula_stuttering by auto
-qed
+qed simp
 
 lemma symrun_interp_set_lifting:
   assumes \<open>set \<Gamma> = set \<Gamma>'\<close>
@@ -222,10 +273,12 @@ theorem symrun_interp_decreases_setinc:
     shows \<open>\<lbrakk>\<lbrakk> \<Gamma> \<rbrakk>\<rbrakk>\<^sub>p\<^sub>r\<^sub>i\<^sub>m \<supseteq> \<lbrakk>\<lbrakk> \<Gamma>' \<rbrakk>\<rbrakk>\<^sub>p\<^sub>r\<^sub>i\<^sub>m\<close>
 proof -
   obtain \<Gamma>\<^sub>r where decompose: \<open>set (\<Gamma> @ \<Gamma>\<^sub>r) = set \<Gamma>'\<close> using assms by auto
-  have \<open>set (\<Gamma> @ \<Gamma>\<^sub>r) = set \<Gamma>'\<close> using assms decompose by blast
+  hence \<open>set (\<Gamma> @ \<Gamma>\<^sub>r) = set \<Gamma>'\<close> using assms by blast
   moreover have \<open>(set \<Gamma>) \<union> (set \<Gamma>\<^sub>r) = set \<Gamma>'\<close> using assms decompose by auto
-  moreover have \<open>\<lbrakk>\<lbrakk> \<Gamma>' \<rbrakk>\<rbrakk>\<^sub>p\<^sub>r\<^sub>i\<^sub>m = \<lbrakk>\<lbrakk> \<Gamma> @ \<Gamma>\<^sub>r \<rbrakk>\<rbrakk>\<^sub>p\<^sub>r\<^sub>i\<^sub>m\<close> using symrun_interp_set_lifting decompose by blast
-  moreover have \<open>\<lbrakk>\<lbrakk> \<Gamma> @ \<Gamma>\<^sub>r \<rbrakk>\<rbrakk>\<^sub>p\<^sub>r\<^sub>i\<^sub>m = \<lbrakk>\<lbrakk> \<Gamma> \<rbrakk>\<rbrakk>\<^sub>p\<^sub>r\<^sub>i\<^sub>m \<inter> \<lbrakk>\<lbrakk> \<Gamma>\<^sub>r \<rbrakk>\<rbrakk>\<^sub>p\<^sub>r\<^sub>i\<^sub>m\<close> by (simp add: symrun_interp_expansion)
+  moreover have \<open>\<lbrakk>\<lbrakk> \<Gamma>' \<rbrakk>\<rbrakk>\<^sub>p\<^sub>r\<^sub>i\<^sub>m = \<lbrakk>\<lbrakk> \<Gamma> @ \<Gamma>\<^sub>r \<rbrakk>\<rbrakk>\<^sub>p\<^sub>r\<^sub>i\<^sub>m\<close>
+    using symrun_interp_set_lifting decompose by blast
+  moreover have \<open>\<lbrakk>\<lbrakk> \<Gamma> @ \<Gamma>\<^sub>r \<rbrakk>\<rbrakk>\<^sub>p\<^sub>r\<^sub>i\<^sub>m = \<lbrakk>\<lbrakk> \<Gamma> \<rbrakk>\<rbrakk>\<^sub>p\<^sub>r\<^sub>i\<^sub>m \<inter> \<lbrakk>\<lbrakk> \<Gamma>\<^sub>r \<rbrakk>\<rbrakk>\<^sub>p\<^sub>r\<^sub>i\<^sub>m\<close>
+    by (simp add: symrun_interp_expansion)
   moreover have \<open>\<lbrakk>\<lbrakk> \<Gamma> \<rbrakk>\<rbrakk>\<^sub>p\<^sub>r\<^sub>i\<^sub>m \<supseteq> \<lbrakk>\<lbrakk> \<Gamma> \<rbrakk>\<rbrakk>\<^sub>p\<^sub>r\<^sub>i\<^sub>m \<inter> \<lbrakk>\<lbrakk> \<Gamma>\<^sub>r \<rbrakk>\<rbrakk>\<^sub>p\<^sub>r\<^sub>i\<^sub>m\<close> by simp
   ultimately show ?thesis by simp
 qed
@@ -246,7 +299,8 @@ qed
 lemma symrun_interp_absorb1:
   assumes \<open>set \<Gamma>\<^sub>1 \<subseteq> set \<Gamma>\<^sub>2\<close>
     shows \<open>\<lbrakk>\<lbrakk> \<Gamma>\<^sub>1 @ \<Gamma>\<^sub>2 \<rbrakk>\<rbrakk>\<^sub>p\<^sub>r\<^sub>i\<^sub>m = \<lbrakk>\<lbrakk> \<Gamma>\<^sub>2 \<rbrakk>\<rbrakk>\<^sub>p\<^sub>r\<^sub>i\<^sub>m\<close>
-by (simp add: Int_absorb1 symrun_interp_decreases_setinc symrun_interp_expansion assms)
+by (simp add: Int_absorb1 symrun_interp_decreases_setinc
+                          symrun_interp_expansion assms)
 
 lemma symrun_interp_absorb2:
   assumes \<open>set \<Gamma>\<^sub>2 \<subseteq> set \<Gamma>\<^sub>1\<close>
